@prefix : <http://www.semanticweb.org/danib/ontologies/2024/3/encuesta_vuelos#> .
@prefix owl: <http://www.w3.org/2002/07/owl#> .
@prefix rdf: <http://www.w3.org/1999/02/22-rdf-syntax-ns#> .
@prefix xml: <http://www.w3.org/XML/1998/namespace> .
@prefix xsd: <http://www.w3.org/2001/XMLSchema#> .
@prefix rdfs: <http://www.w3.org/2000/01/rdf-schema#> .
@base <http://www.semanticweb.org/danib/ontologies/2024/3/encuesta_vuelos#> .

<http://www.semanticweb.org/danib/ontologies/2024/3/encuesta_vuelos> rdf:type owl:Ontology ;
                                                                      rdfs:comment """1. Descripción

Esta ontología modela las respuestas de encuestas de satisfacción de clientes de aerolíneas, enfocándose en Qatar Airways y Ryanair.

2. Propósito y Caso de uso

Propósito: Facilitar el análisis y comparación de la satisfacción del cliente entre diferentes aerolíneas. 
Caso de Uso: Analizar las tendencias de satisfacción en servicios a bordo entre Qatar Airways y Ryanair.

3. Requerimientos

- ¿Cuál es el promedio de satisfacción general para Qatar Airways?
- ¿Cómo se comparan las tasas de satisfacción del servicio a bordo entre Qatar Airways y Ryanair?
- ¿Qué factores están más correlacionados con la insatisfacción del cliente en Ryanair?
- ¿Hay diferencias estacionales en la satisfacción del cliente en ambas aerolíneas?

4, Especificaciones

Los datos provienen de encuestas de satisfacción disponibles en Kaggle para Qatar Airways y Ryanair, presentadas en formato CSV.""" ;
                                                                      rdfs:label "Ontología de Encuestas de Satisfacción de Vuelos" .

#################################################################
#    Object Properties
#################################################################

###  http://www.semanticweb.org/danib/ontologies/2024/3/encuesta_vuelos#fliesFrom
:fliesFrom rdf:type owl:ObjectProperty ;
           rdfs:domain :Flight ;
           rdfs:range :Airport .


###  http://www.semanticweb.org/danib/ontologies/2024/3/encuesta_vuelos#hasFlown
:hasFlown rdf:type owl:ObjectProperty ;
          rdfs:domain :Customer ;
          rdfs:range :Flight .


###  http://www.semanticweb.org/danib/ontologies/2024/3/encuesta_vuelos#hasReviewed
:hasReviewed rdf:type owl:ObjectProperty ;
             rdfs:domain :Customer ;
             rdfs:range :Review .


###  http://www.semanticweb.org/danib/ontologies/2024/3/encuesta_vuelos#operatesFlight
:operatesFlight rdf:type owl:ObjectProperty ;
                rdfs:domain :Airline ;
                rdfs:range :Flight .


#################################################################
#    Data properties
#################################################################

###  http://www.semanticweb.org/danib/ontologies/2024/3/encuesta_vuelos#aircraftType
:aircraftType rdf:type owl:DatatypeProperty ;
              rdfs:domain :Flight ;
              rdfs:range xsd:string .


###  http://www.semanticweb.org/danib/ontologies/2024/3/encuesta_vuelos#customerCountry
:customerCountry rdf:type owl:DatatypeProperty ;
                 rdfs:domain :Customer ;
                 rdfs:range xsd:string .


###  http://www.semanticweb.org/danib/ontologies/2024/3/encuesta_vuelos#flightDate
:flightDate rdf:type owl:DatatypeProperty ;
            rdfs:domain :Flight ;
            rdfs:range xsd:string .


###  http://www.semanticweb.org/danib/ontologies/2024/3/encuesta_vuelos#reviewDate
:reviewDate rdf:type owl:DatatypeProperty ;
            rdfs:domain :Review ;
            rdfs:range xsd:string .


###  http://www.semanticweb.org/danib/ontologies/2024/3/encuesta_vuelos#reviewRating
:reviewRating rdf:type owl:DatatypeProperty ;
              rdfs:domain :Review ;
              rdfs:range xsd:integer .


###  http://www.semanticweb.org/danib/ontologies/2024/3/encuesta_vuelos#seatType
:seatType rdf:type owl:DatatypeProperty ;
          rdfs:domain :Flight ;
          rdfs:range xsd:string .


#################################################################
#    Classes
#################################################################

###  http://www.semanticweb.org/danib/ontologies/2024/3/encuesta_vuelos#Aircraft
:Aircraft rdf:type owl:Class ;
          rdfs:comment "Refers to any kind of airplane used in commercial flights." .


###  http://www.semanticweb.org/danib/ontologies/2024/3/encuesta_vuelos#Airline
:Airline rdf:type owl:Class ;
         rdfs:comment "An organization providing air transport services for traveling passengers and freight." .


###  http://www.semanticweb.org/danib/ontologies/2024/3/encuesta_vuelos#Airport
:Airport rdf:type owl:Class ;
         rdfs:comment "Represents an airport, which is a location where flights take off and land." .


###  http://www.semanticweb.org/danib/ontologies/2024/3/encuesta_vuelos#AverageRating
:AverageRating rdf:type owl:Class ;
               rdfs:subClassOf :Rating ;
               rdfs:comment "Indicates a moderate level of satisfaction in customer reviews." .


###  http://www.semanticweb.org/danib/ontologies/2024/3/encuesta_vuelos#BusinessTraveller
:BusinessTraveller rdf:type owl:Class ;
                   rdfs:subClassOf :Review ;
                   rdfs:comment "A customer traveling for business purposes." .


###  http://www.semanticweb.org/danib/ontologies/2024/3/encuesta_vuelos#CabinStaffService
:CabinStaffService rdf:type owl:Class ;
                   rdfs:subClassOf :ServiceAspect ;
                   rdfs:comment "Refers to the quality of service provided by the airline's cabin staff." .


###  http://www.semanticweb.org/danib/ontologies/2024/3/encuesta_vuelos#CoupleLeisure
:CoupleLeisure rdf:type owl:Class ;
               rdfs:subClassOf :Review ;
               rdfs:comment "Leisure travelers flying as a couple." .


###  http://www.semanticweb.org/danib/ontologies/2024/3/encuesta_vuelos#Customer
:Customer rdf:type owl:Class ;
          owl:equivalentClass [ rdf:type owl:Restriction ;
                                owl:onProperty :hasReviewed ;
                                owl:minQualifiedCardinality "1"^^xsd:nonNegativeInteger ;
                                owl:onClass :Customer
                              ] ;
          rdfs:comment "An individual who purchases air travel service from airlines." .


###  http://www.semanticweb.org/danib/ontologies/2024/3/encuesta_vuelos#ExcellentRating
:ExcellentRating rdf:type owl:Class ;
                 rdfs:subClassOf :Rating ;
                 rdfs:comment "Indicates an exceptional level of satisfaction in customer reviews." .


###  http://www.semanticweb.org/danib/ontologies/2024/3/encuesta_vuelos#FamilyLeisure
:FamilyLeisure rdf:type owl:Class ;
               rdfs:subClassOf :Review ;
               rdfs:comment "Families traveling together for leisure purposes." .


###  http://www.semanticweb.org/danib/ontologies/2024/3/encuesta_vuelos#Flight
:Flight rdf:type owl:Class ;
        rdfs:comment "A journey made by an airplane from one airport to another." .


###  http://www.semanticweb.org/danib/ontologies/2024/3/encuesta_vuelos#FoodBeverages
:FoodBeverages rdf:type owl:Class ;
               rdfs:subClassOf :ServiceAspect ;
               rdfs:comment "Refers to the quality and variety of food and drinks offered during the flight." .


###  http://www.semanticweb.org/danib/ontologies/2024/3/encuesta_vuelos#GoodRating
:GoodRating rdf:type owl:Class ;
            rdfs:subClassOf :Rating ;
            rdfs:comment "Indicates a good level of satisfaction in customer reviews." .


###  http://www.semanticweb.org/danib/ontologies/2024/3/encuesta_vuelos#GroundService
:GroundService rdf:type owl:Class ;
               rdfs:subClassOf :ServiceAspect ;
               rdfs:comment "Refers to the services provided on the ground, such as check-in and baggage handling." .


###  http://www.semanticweb.org/danib/ontologies/2024/3/encuesta_vuelos#GroupLeisure
:GroupLeisure rdf:type owl:Class ;
              rdfs:subClassOf :Review ;
              rdfs:comment "Groups of people traveling together for leisure purposes." .


###  http://www.semanticweb.org/danib/ontologies/2024/3/encuesta_vuelos#InflightEntertainment
:InflightEntertainment rdf:type owl:Class ;
                       rdfs:subClassOf :ServiceAspect ;
                       rdfs:comment "Entertainment options available to passengers during the flight." .


###  http://www.semanticweb.org/danib/ontologies/2024/3/encuesta_vuelos#PoorRating
:PoorRating rdf:type owl:Class ;
            rdfs:subClassOf :Rating ;
            rdfs:comment "Indicates a low level of satisfaction in customer reviews." .


###  http://www.semanticweb.org/danib/ontologies/2024/3/encuesta_vuelos#QatarAirways
:QatarAirways rdf:type owl:Class ;
              rdfs:subClassOf :Aircraft ;
              owl:disjointWith :Ryanair ;
              rdfs:comment "The state-owned flag carrier of Qatar, providing international flights." .


###  http://www.semanticweb.org/danib/ontologies/2024/3/encuesta_vuelos#Rating
:Rating rdf:type owl:Class ;
        rdfs:comment "Represents the ratings given to airlines based on customer reviews." .


###  http://www.semanticweb.org/danib/ontologies/2024/3/encuesta_vuelos#Review
:Review rdf:type owl:Class ;
        owl:equivalentClass [ rdf:type owl:Restriction ;
                              owl:onProperty :reviewRating ;
                              owl:qualifiedCardinality "1"^^xsd:nonNegativeInteger ;
                              owl:onDataRange xsd:integer
                            ] ;
        rdfs:comment "A customer's evaluation or assessment of their flight experience." .


###  http://www.semanticweb.org/danib/ontologies/2024/3/encuesta_vuelos#Ryanair
:Ryanair rdf:type owl:Class ;
         rdfs:subClassOf :Aircraft ;
         rdfs:comment "An Irish low-cost airline headquartered in Dublin, known for its budget travel services." .


###  http://www.semanticweb.org/danib/ontologies/2024/3/encuesta_vuelos#SeatComfort
:SeatComfort rdf:type owl:Class ;
             rdfs:subClassOf :ServiceAspect ;
             rdfs:comment "Refers to how comfortable the seating arrangements are on the flight." .


###  http://www.semanticweb.org/danib/ontologies/2024/3/encuesta_vuelos#ServiceAspect
:ServiceAspect rdf:type owl:Class ;
               rdfs:comment "Different aspects of airline service that are rated in reviews, such as seat comfort or food quality." .


###  http://www.semanticweb.org/danib/ontologies/2024/3/encuesta_vuelos#SoloLeisure
:SoloLeisure rdf:type owl:Class ;
             rdfs:subClassOf :Review ;
             rdfs:comment "Individuals traveling alone for leisure purposes." .


###  http://www.semanticweb.org/danib/ontologies/2024/3/encuesta_vuelos#Verified
:Verified rdf:type owl:Class ;
          rdfs:subClassOf :Review ;
          rdfs:comment "Indicates whether a review has been verified as authentic." .


###  http://www.semanticweb.org/danib/ontologies/2024/3/encuesta_vuelos#WifiConnectivity
:WifiConnectivity rdf:type owl:Class ;
                  rdfs:subClassOf :ServiceAspect ;
                  rdfs:comment "Refers to the availability and quality of WiFi connection aboard the aircraft." .


#################################################################
#    Individuals
#################################################################

###  http://www.semanticweb.org/danib/ontologies/2024/3/encuesta_vuelos#CustomerJohnDoe
:CustomerJohnDoe rdf:type owl:NamedIndividual ,
                          :Customer ;
                 :customerCountry "USA" ;
                 rdfs:comment "A frequent business traveler who uses various airlines for international travel." .


###  http://www.semanticweb.org/danib/ontologies/2024/3/encuesta_vuelos#DohaAirport
:DohaAirport rdf:type owl:NamedIndividual ,
                      :Airport ;
             rdfs:comment "The international airport for Doha, Qatar, serving as the primary hub for Qatar Airways." ;
             rdfs:label "Hamad International Airport" .


###  http://www.semanticweb.org/danib/ontologies/2024/3/encuesta_vuelos#ExcellentRatingFiveStars
:ExcellentRatingFiveStars rdf:type owl:NamedIndividual ,
                                   :ExcellentRating ,
                                   :Rating ;
                          rdfs:label "Excellent Rating" .


###  http://www.semanticweb.org/danib/ontologies/2024/3/encuesta_vuelos#FlightQR905
:FlightQR905 rdf:type owl:NamedIndividual ,
                      :Flight ;
             rdfs:comment "A daily flight from Doha to London operated by Qatar Airways." .


###  http://www.semanticweb.org/danib/ontologies/2024/3/encuesta_vuelos#Qatar_Airways
:Qatar_Airways rdf:type owl:NamedIndividual ,
                        :Airline ;
               rdfs:comment "A major international airline based in Doha, known for its high service quality" .


###  http://www.semanticweb.org/danib/ontologies/2024/3/encuesta_vuelos#ReviewJohnDoeQR905
:ReviewJohnDoeQR905 rdf:type owl:NamedIndividual ,
                             :Review ;
                    :reviewDate "2024-04-01" ;
                    :reviewRating 5 ;
                    rdfs:comment "John Doe's review of his flight from Doha to London on Qatar Airways." ;
                    rdfs:label "Review of Flight QR905 by John Doe" .


#################################################################
#    General axioms
#################################################################

[ rdf:type owl:AllDisjointClasses ;
  owl:members ( :AverageRating
                :ExcellentRating
                :GoodRating
                :PoorRating
              )
] .


[ rdf:type owl:AllDisjointClasses ;
  owl:members ( :BusinessTraveller
                :CoupleLeisure
                :FamilyLeisure
                :GroupLeisure
                :SoloLeisure
                :Verified
              )
] .


[ rdf:type owl:AllDisjointClasses ;
  owl:members ( :CabinStaffService
                :FoodBeverages
                :GroundService
                :InflightEntertainment
                :SeatComfort
                :WifiConnectivity
              )
] .


###  Generated by the OWL API (version 5.1.18) https://github.com/owlcs/owlapi/
